theories/IL/ListToStmt.v
@@ -1,0 +1,77 @@
+Require Import Util MoreList Get Option OptionMap.
+Require Import Var IL AppExpFree.
+
+Fixpoint list_to_stmt (xl: list var) (Y : list op) (s : stmt) : stmt :=
+  match xl, Y with
+  | x::xl, e :: Y => stmtLet x  (Operation e) (list_to_stmt xl Y s)
+  | _, _ => s
+  end.
+
+Lemma list_to_stmt_correct L E s xl Y vl
+: length xl = length Y
+  -> omap (op_eval E) Y = Some vl
+  -> NoDupA _eq xl
+  -> disj (of_list xl) (list_union (List.map Op.freeVars Y))
+  -> star2 F.step (L, E, list_to_stmt xl Y s) nil
+          (L, update_with_list' xl (List.map Some vl) E, s).
+Proof.
+  intros Len Eq Uni Disj.
+  length_equify.
+  general induction Len; simpl in * |- *; eauto using star2_refl.
+  - simpl in *. monad_inv Eq.
+    eapply star2_silent.
+    econstructor; eauto.
+    rewrite list_union_start_swap in Disj.
+    eapply IHLen; eauto.
+    eapply omap_op_eval_agree; eauto.
+    symmetry. eapply agree_on_update_dead; [|reflexivity].
+    eauto with cset.
+    eapply disj_incl; eauto with cset.
+Qed.
+
+Lemma list_to_stmt_crash L E xl Y s
+: length xl = length Y
+  -> omap (op_eval E) Y = None
+  -> NoDupA _eq xl
+  -> disj (of_list xl) (list_union (List.map Op.freeVars Y))
+  -> exists σ, star2 F.step (L, E, list_to_stmt xl Y s) nil σ
+         /\ state_result σ = None
+         /\ normal2 F.step σ.
+Proof.
+  intros. eapply length_length_eq in H.
+  general induction H; simpl in * |- *.
+  - monad_inv H0.
+    + eexists. split. eapply star2_refl.
+      split; eauto. stuck2.
+    + rewrite list_union_start_swap in H2.
+      edestruct (IHlength_eq L (E [x <- Some x0])); eauto.
+      * eapply omap_op_eval_agree; eauto. symmetry.
+        eapply agree_on_update_dead; [|reflexivity].
+        intro. eapply (H2 x); eauto with cset.
+      * eapply disj_incl; eauto with cset.
+      * dcr. eexists. split; eauto.
+        eapply star2_silent.
+        econstructor; eauto. eauto.
+Qed.
+
+Lemma list_to_stmt_app_expfree  ZL Y Y' l
+  : (forall n e, get Y' n e -> isVar e)
+    -> app_expfree (list_to_stmt ZL Y (stmtApp l Y')).
+Proof.
+  general induction Y; destruct ZL; destruct Y'; simpl;
+    econstructor; intros; inv_get; isabsurd; eauto using isVar.
+Qed.
+
+
+Lemma list_to_stmt_freeVars xl Y s (Len:❬xl❭ = ❬Y❭)
+      (Disj:disj (of_list xl) (list_union (Op.freeVars ⊝ Y)))
+  : freeVars (list_to_stmt xl Y s) [=] list_union (Op.freeVars ⊝ Y) ∪ (freeVars s \ of_list xl).
+Proof.
+  general induction Len; simpl in *.
+  - cset_tac.
+  - setoid_rewrite list_union_start_swap.
+    setoid_rewrite list_union_start_swap in Disj.
+    rewrite IHLen.
+    clear IHLen. cset_tac.
+    eapply disj_incl; eauto with cset.
+Qed.
