theories/Infra/ReplaceIf.v
@@ -1,0 +1,42 @@
+Require Import Util MoreList Get Option OptionMap Filter.
+
+Set Implicit Arguments.
+
+Fixpoint replace_if X (p:X -> bool) (L:list X) (L':list X) :=
+  match L with
+  | x::L => if p x then
+              match L' with
+              | y::L' => y::replace_if p L L'
+              | _ => nil
+              end
+            else
+              x::replace_if p L L'
+  | _ => nil
+  end.
+
+Lemma replace_if_get_inv X (p:X -> bool) L L' n x
+  : get (replace_if p L L') n x
+    -> exists l , get L n l /\
+            ((p l /\ exists l' n', get L' n' l' /\ x = l')
+              \/ (~ p l /\ x = l)).
+Proof.
+  intros; general induction L; destruct L'; simpl in *; isabsurd.
+  - cases in H; isabsurd. inv H.
+    + exists x; split; eauto using get.
+      right; split; eauto. rewrite <- Heq. eauto.
+    + edestruct IHL; eauto; dcr.
+      eexists; split; eauto using get.
+  - cases in H; isabsurd.
+    + inv H.
+      * eexists; split; eauto using get.
+        left. rewrite <- Heq; eauto using get.
+      * edestruct IHL; eauto using get; dcr.
+        eexists; split; eauto using get.
+        destruct H2; dcr; isabsurd. left; eauto 20 using get.
+        right; eauto using get.
+    + inv H.
+      * eexists; split; eauto using get.
+        right. rewrite <- Heq; eauto using get.
+      * edestruct IHL; eauto; dcr.
+        eexists; split; eauto using get.
+Qed.
